concurrency/framework/GlinearSeq.s.dfy
@@ -1,0 +1,22 @@
+module GlinearSeq {
+  type {:extern} glseq<V>
+  {
+    function {:extern} len() : nat
+
+    predicate {:extern} has(i: nat)
+    requires i < len()
+
+    function {:extern} get(i: nat) : V
+    requires i < len() && has(i)
+  }
+
+  glinear method {:extern} glseq_take<V>(glinear g: glseq<V>, ghost i: nat)
+  returns (glinear g': glseq<V>, glinear v': V)
+  requires i < g.len()
+  requires g.has(i)
+  ensures v' == g.get(i)
+  ensures g'.len() == g.len()
+  ensures forall j | 0 <= j < g.len() :: j != i ==> !g.has(j) ==> !g'.has(j)
+  ensures forall j | 0 <= j < g.len() ::
+      j != i ==> g.has(j) ==> g'.has(j) && g'.get(j) == g.get(j)
+}
